Split up GF25519Reflective.Common: faster+parallel
After    | File Name                                     | Before   || Change
--------------------------------------------------------------------------------
2m53.12s | Total                                         | 2m52.26s || +0m00.85s
--------------------------------------------------------------------------------
0m01.38s | Specific/GF25519Reflective/Common             | 0m43.51s || -0m42.12s
0m14.82s | Specific/GF25519Reflective/CommonBinOp        |   N/A    || +0m14.82s
0m10.91s | Specific/GF25519Reflective/CommonUnOp         |   N/A    || +0m10.91s
0m10.44s | Specific/GF25519Reflective/CommonUnOpWireToFE |   N/A    || +0m10.43s
0m06.42s | Specific/GF25519Reflective/CommonUnOpFEToWire |   N/A    || +0m06.41s
1m18.24s | Experiments/Ed25519                           | 1m18.57s || -0m00.32s
0m07.97s | Specific/GF25519Reflective/Reified/Mul        | 0m08.45s || -0m00.47s
0m07.89s | Specific/GF25519Reflective/Reified/Freeze     | 0m07.84s || +0m00.04s
0m06.87s | Specific/GF25519Reflective                    | 0m06.92s || -0m00.04s
0m03.53s | Specific/GF25519Reflective/Reified/CarrySub   | 0m03.63s || -0m00.10s
0m03.27s | Specific/GF25519Reflective/Reified/CarryAdd   | 0m03.28s || -0m00.00s
0m03.18s | Specific/GF25519Reflective/Reified/CarryOpp   | 0m03.15s || +0m00.03s
0m02.24s | Specific/GF25519Reflective/Reified/Unpack     | 0m02.21s || +0m00.03s
0m02.19s | Specific/GF25519Reflective/Reified/Pack       | 0m02.28s || -0m00.08s
0m02.16s | Specific/GF25519Reflective/Reified/Sub        | 0m02.15s || +0m00.01s
0m02.14s | Specific/GF25519Bounded                       | 0m02.07s || +0m00.07s
0m02.07s | Experiments/Ed25519Extraction                 | 0m02.16s || -0m00.09s
0m01.99s | Specific/GF25519Reflective/Reified/Add        | 0m01.81s || +0m00.17s
0m01.82s | Specific/GF25519Reflective/Reified/Opp        | 0m01.78s || +0m00.04s
0m01.76s | Specific/GF25519Reflective/Reified/GeModulus  | 0m01.71s || +0m00.05s
0m00.97s | Specific/GF25519Reflective/CommonUnOpFEToZ    |   N/A    || +0m00.97s
0m00.86s | Specific/GF25519Reflective/Reified            | 0m00.75s || +0m00.10s

src/Specific/GF25519Reflective/Reified/rebuild-reified.py
@@ -25,7 +25,7 @@ Definition r%(lname)sW_correct_and_bounded
        match proof_admitted with end match proof_admitted with end.
 """ % locals()
     with open(name.replace('_', '') + '.v', 'w') as f:
-        f.write(r"""Require Import Crypto.Specific.GF25519Reflective.Common.
+        f.write(r"""Require Import Crypto.Specific.GF25519Reflective.Common%(uopkind)s.
 
 Definition r%(lname)sZ_sig : rexpr_%(lopkind)s_sig %(lname)s. Proof. reify_sig. Defined.
 Definition r%(lname)sW := Eval vm_compute in rword_of_Z r%(lname)sZ_sig.
