src/Specific/GF25519Reflective/Reified/GeModulus.v
@@ -1,4 +1,4 @@
-Require Import Crypto.Specific.GF25519Reflective.Common.
+Require Import Crypto.Specific.GF25519Reflective.CommonUnOpFEToZ.
 
 Definition rge_modulusZ_sig : rexpr_unop_FEToZ_sig ge_modulus. Proof. reify_sig. Defined.
 Definition rge_modulusW := Eval vm_compute in rword_of_Z rge_modulusZ_sig.
