src/Specific/GF25519Reflective/Reified/Pack.v
@@ -1,4 +1,4 @@
-Require Import Crypto.Specific.GF25519Reflective.Common.
+Require Import Crypto.Specific.GF25519Reflective.CommonUnOpFEToWire.
 
 Definition rpackZ_sig : rexpr_unop_FEToWire_sig pack. Proof. reify_sig. Defined.
 Definition rpackW := Eval vm_compute in rword_of_Z rpackZ_sig.
